Setlec/Verify/PairM.lean
@@ -500,18 +500,6 @@ theorem proofIrrel_snd_proj (d : Nat) (a b : Expr) :
   unfold proofIrrel
   snd_tac
 
-theorem pairEtaCert_fst_proj (d : Nat) (a b : Expr) :
-    (pairEtaCert mode (pairFns r₁ r₂ h) env d a b).val.1 =
-      pairEtaCert mode r₁ env d a b := by
-  unfold pairEtaCert
-  fst_tac
-
-theorem pairEtaCert_snd_proj (d : Nat) (a b : Expr) :
-    (pairEtaCert mode (pairFns r₁ r₂ h) env d a b).val.2 =
-      pairEtaCert mode r₂ env d a b := by
-  unfold pairEtaCert
-  snd_tac
-
 theorem structEtaCertWith_fst_proj (d : Nat) (a b wtb : Expr) :
     (structEtaCertWith mode (pairFns r₁ r₂ h) env d a b wtb).val.1 =
       structEtaCertWith mode r₁ env d a b wtb := by
@@ -570,7 +558,6 @@ macro "fst_step2" : tactic =>
     | (rw [reduceNat_fst_proj])
     | (rw [ensureSort_fst_proj])
     | (rw [proofIrrel_fst_proj])
-    | (rw [pairEtaCert_fst_proj])
     | (rw [structEtaCertWith_fst_proj])
     | (rw [structUnitCert_fst_proj])
     | (rw [etaCert_fst_proj])
@@ -595,7 +582,6 @@ macro "snd_step2" : tactic =>
     | (rw [reduceNat_snd_proj])
     | (rw [ensureSort_snd_proj])
     | (rw [proofIrrel_snd_proj])
-    | (rw [pairEtaCert_snd_proj])
     | (rw [structEtaCertWith_snd_proj])
     | (rw [structUnitCert_snd_proj])
     | (rw [etaCert_snd_proj])
@@ -746,7 +732,6 @@ macro "fst_step3" : tactic =>
     | (rw [reduceNat_fst_proj])
     | (rw [ensureSort_fst_proj])
     | (rw [proofIrrel_fst_proj])
-    | (rw [pairEtaCert_fst_proj])
     | (rw [structEtaCertWith_fst_proj])
     | (rw [structUnitCert_fst_proj])
     | (rw [etaCert_fst_proj])
@@ -775,7 +760,6 @@ macro "snd_step3" : tactic =>
     | (rw [reduceNat_snd_proj])
     | (rw [ensureSort_snd_proj])
     | (rw [proofIrrel_snd_proj])
-    | (rw [pairEtaCert_snd_proj])
     | (rw [structEtaCertWith_snd_proj])
     | (rw [structUnitCert_snd_proj])
     | (rw [etaCert_snd_proj])
@@ -832,7 +816,6 @@ macro "fst_core4" x:tactic : tactic =>
     | (rw [reduceNat_fst_proj])
     | (rw [ensureSort_fst_proj])
     | (rw [proofIrrel_fst_proj])
-    | (rw [pairEtaCert_fst_proj])
     | (rw [structEtaCertWith_fst_proj])
     | (rw [structUnitCert_fst_proj])
     | (rw [etaCert_fst_proj])
@@ -882,7 +865,6 @@ macro "snd_core4" x:tactic : tactic =>
     | (rw [reduceNat_snd_proj])
     | (rw [ensureSort_snd_proj])
     | (rw [proofIrrel_snd_proj])
-    | (rw [pairEtaCert_snd_proj])
     | (rw [structEtaCertWith_snd_proj])
     | (rw [structUnitCert_snd_proj])
     | (rw [etaCert_snd_proj])
